theories/SLFExtra.v
@@ -1112,6 +1112,59 @@ Qed.
 
 
 (* ########################################################### *)
+(** ** Specification of [val_get_header] and [val_array_length] *)
+
+Lemma eval_get_header_sep : forall s s2 p k,
+  s = Fmap.union (Fmap.single p (hval_header k)) s2 ->
+  eval s (val_get_header (val_loc p)) s (val_int k).
+Proof using.
+  introv ->. forwards Dv: Fmap.indom_single p (hval_header k).
+  applys eval_get_header.
+  { applys~ Fmap.indom_union_l. }
+  { rewrite~ Fmap.read_union_l. rewrite~ Fmap.read_single. }
+Qed.
+
+Lemma hoare_get_header : forall H k p,
+  hoare (val_get_header p)
+    ((p ~~> hval_header k) \* H)
+    (fun r => \[r = k] \* (p ~~> hval_header k) \* H).
+Proof using.
+  intros. intros s K0. exists s (val_int k). split.
+  { destruct K0 as (s1&s2&P1&P2&D&U).
+    lets E1: hsingle_inv P1. subst s1. applys eval_get_header_sep U. }
+  { rewrite~ hstar_hpure. }
+Qed.
+
+Lemma triple_get_header' : forall H k p,
+  triple (val_get_header p)
+    ((p ~~> hval_header k) \* H)
+    (fun r => \[r = k] \* (p ~~> hval_header k) \* H).
+Proof using.
+  intros. unfold triple. intros H'. applys hoare_conseq hoare_get_header; xsimpl~.
+Qed.
+
+Lemma triple_get_header : forall k p,
+  triple (val_get_header p)
+    (header k p)
+    (fun r => \[r = k] \* header k p).
+Proof using.
+  intros. unfold header. rewrite hstar_comm. applys triple_hpure. intros N.
+  applys triple_conseq triple_get_header'. { xsimpl. } { xsimpl; auto. }
+Qed.
+
+Definition val_array_length : val := val_get_header.
+
+Lemma triple_array_length : forall L p,
+  triple (val_array_length p)
+    (harray L p)
+    (fun r => \[r = length L] \* harray L p).
+Proof using.
+  intros. unfold harray. applys triple_conseq_frame triple_get_header.
+  { xsimpl. } { xsimpl. auto. }
+Qed.
+
+
+(* ########################################################### *)
 (** ** Encoding of [val_array_get] and [val_array_set] *)
 
 Module Export ArrayAccessDef.
